de bruijn renumbering fun

src/grw.v
@@ -196,24 +196,21 @@ Definition expr_type '((_, p2) : expr) : type := op_type p2.
    - Can refer to universally-quantified variables as free de Bruijn indices
 *)
 Fixpoint interp_bindings (ctxt : type) (ctx : interp_type ctxt)
-         (p1 : list operation)
+         (p : list operation)
          (tk : type) (k : forall ctxt : type, interp_type ctxt -> M tk)
-         {struct p1} : (M tk) :=
-  match p1 with
+         {struct p} : (M tk) :=
+  match p with
   | nil => k ctxt ctx
-  | cons o p1 =>
+  | cons o p =>
     Mbind (interp_op_silent ctxt ctx o)
-          (fun x => interp_bindings (op_type o * ctxt) (x, ctx) p1 tk k)
+          (fun x => interp_bindings (op_type o * ctxt) (x, ctx) p tk k)
   end.
 
 Definition interp_expr (ctxt : type) (ctx : interp_type ctxt)
            (e : expr) : M (expr_type e) :=
-  let '(p1, p2) := e in
-  interp_bindings ctxt ctx p1 (op_type p2)
-                  (fun ctxt ctx => interp_op_silent ctxt ctx p2).
-
-Definition interp_closed_expr (e : expr) : M (expr_type e) :=
-  interp_expr tunit tt e.
+  let '(p, o) := e in
+  interp_bindings ctxt ctx p (op_type o)
+                  (fun ctxt ctx => interp_op_silent ctxt ctx o).
 
 Example reflection_example :
   let x := ((op_unit
@@ -222,12 +219,254 @@ Example reflection_example :
                :: (op_app coin (ref_index 1))
                :: nil),
             (op_retapp xor' (ref_pair (ref_index 0) (ref_index 1)))) in
-  let y := interp_closed_expr x in
-  {z & Comp_eq y z}.
+  {z | forall ctxt ctx,
+      let y := interp_expr ctxt ctx x in
+      Comp_eq y z}.
 Proof.
-  intros x y; subst x y.
+  intros x.
   eexists.
+  intros.
+  subst x y.
   cbv - [Vector.nth xorb Comp_eq].
   repeat setoid_rewrite Bind_unused.
   reflexivity.
 Defined.
+
+Lemma Mequiv_Mbind (t1 t2 : type)
+      (c1 c1' : M t1) (c2 c2' : interp_type t1 -> M t2) :
+  Mequiv c1 c1' ->
+  (forall x, Mequiv (c2 x) (c2' x)) ->
+  Mequiv (Mbind c1 c2) (Mbind c1' c2').
+Proof. cbv [Mequiv Mbind]; intros; eapply Proper_Bind; eauto. Qed.
+
+Lemma interp_bindings_app ctxt (ctx : interp_type ctxt)
+      (p1 p2 : list operation) tk (k : forall ctxt, interp_type ctxt -> M tk) :
+  Mequiv
+    (interp_bindings ctxt ctx (p1 ++ p2) tk k)
+    (interp_bindings ctxt ctx p1 tk
+                     (fun ctxt ctx => interp_bindings ctxt ctx p2 tk k)).
+Proof.
+  revert ctxt ctx p2 tk k;
+    induction p1 as [|o p1]; intros ctxt ctx p2 tk k;
+      [reflexivity|].
+  cbn [interp_bindings app].
+  eapply Mequiv_Mbind; [reflexivity | eauto].
+Qed.
+
+Definition continuation_compat tk
+           (k k' : forall ctxt : type, interp_type ctxt -> M tk) : Prop :=
+  forall ctxt (ctx : interp_type ctxt),
+    Mequiv (k ctxt ctx) (k' ctxt ctx).
+
+Fixpoint renumber_ref (f : nat -> nat) (r : ref) : ref :=
+  match r with
+  | ref_index n => ref_index (f n)
+  | ref_pair r1 r2 => ref_pair (renumber_ref f r1) (renumber_ref f r2)
+  end.
+
+Definition renumber_op (f : nat -> nat) (o : operation) : operation :=
+  match o with
+  | op_unit => op_unit
+  | op_app c r => op_app c (renumber_ref f r)
+  | op_retapp c r => op_retapp c (renumber_ref f r)
+  end.
+
+Fixpoint optsub (n m : nat) {struct m} : option nat :=
+  match m with
+  | 0 => Some n
+  | S m => match n with
+           | 0 => None
+           | S n => optsub n m
+           end
+  end.
+
+Local Notation "a -? b" := (optsub a b) (left associativity, at level 50).
+
+Definition offset_renumbering (offset : nat)
+           (f : nat -> nat) (n : nat) : nat :=
+  match n -? offset with
+  | Some k => offset + (f k)
+  | None => n
+  end.
+
+Fixpoint renumber_bindings (f : nat -> nat) (p : list operation)
+  : list operation :=
+  match p with
+  | nil => nil
+  | cons o p =>
+    cons (renumber_op f o)
+         (renumber_bindings (offset_renumbering 1 f) p)
+  end.
+
+Section RenumberExt.
+  Context (f f' : nat -> nat)
+          (H : forall n, f n = f' n).
+  Lemma renumber_ref_ext r : renumber_ref f r = renumber_ref f' r.
+  Proof. induction r; cbn [renumber_ref]; congruence. Qed.
+  Lemma renumber_op_ext o : renumber_op f o = renumber_op f' o.
+  Proof.
+    induction o; cbn [renumber_op]; try rewrite renumber_ref_ext; congruence.
+  Qed.
+End RenumberExt.
+Lemma renumber_bindings_ext f f' p :
+  (forall n, f n = f' n) ->
+  renumber_bindings f p = renumber_bindings f' p.
+Proof.
+  revert f f'; induction p as [|o p]; eauto.
+  intros; cbn [renumber_bindings].
+  f_equal; eauto using renumber_op_ext.
+  apply IHp.
+  intros n.
+  cbv [offset_renumbering]; destruct (optsub n 1); congruence.
+Qed.
+
+Lemma offset_renumbering_plus a b n f :
+  offset_renumbering (a + b) f n =
+  offset_renumbering a (offset_renumbering b f) n.
+Proof.
+  revert b n; induction a; intros b n; eauto.
+  cbv [offset_renumbering] in *.
+  rewrite PeanoNat.Nat.add_succ_l.
+  cbn [optsub].
+  destruct n; eauto.
+  specialize (IHa b n).
+  destruct (n -? (a + b)), (n -? a); omega.
+Qed.
+
+Lemma renumber_bindings_app (f : nat -> nat) (p1 p2 : list operation) :
+  renumber_bindings f (p1 ++ p2) =
+  (renumber_bindings f p1)
+    ++ renumber_bindings (offset_renumbering (length p1) f) p2.
+Proof.
+  revert f; induction p1; intros f; eauto.
+  repeat (rewrite <- app_comm_cons ||
+          cbn [renumber_bindings offset_renumbering optsub length]).
+  f_equal.
+  rewrite <-(Nat.add_1_r (length p1)).
+  erewrite (renumber_bindings_ext (offset_renumbering (length p1 + 1) f));
+    eauto using offset_renumbering_plus.
+Qed.
+
+Definition context_renumbered (f : nat -> nat)
+           ctxt (ctx : interp_type ctxt)
+           ctxt' (ctx' : interp_type ctxt') : Prop :=
+  forall i t, lookup ctxt' ctx' (f i) t = lookup ctxt ctx i t.
+
+Lemma context_renumbered_ext f1 f2 ctxt ctx ctxt' ctx' :
+  (forall n, f1 n = f2 n) ->
+  context_renumbered f1 ctxt ctx ctxt' ctx' <->
+  context_renumbered f2 ctxt ctx ctxt' ctx'.
+Proof. intuition congruence. Qed.
+
+Definition continuation_renumbered (f : nat -> nat) tk
+           (k k' : forall ctxt : type, interp_type ctxt -> M tk) :=
+  forall ctxt (ctx : interp_type ctxt) ctxt' (ctx' : interp_type ctxt'),
+    context_renumbered f ctxt ctx ctxt' ctx' ->
+    Mequiv (k ctxt ctx) (k' ctxt' ctx').
+
+Local Instance continuation_renumbered_Mequiv f tk :
+  Proper ((forall_relation
+             (fun ctxt => pointwise_relation (interp_type ctxt) Mequiv)
+             ==>
+             (forall_relation
+                (fun ctxt => pointwise_relation (interp_type ctxt) Mequiv))
+             ==> iff)) (continuation_renumbered f tk).
+Proof.
+  cbv [Proper respectful forall_relation pointwise_relation Basics.impl].
+  cbv [continuation_renumbered].
+  intros; split; intros.
+  - etransitivity; [symmetry; eauto|];
+      etransitivity; [|eauto]; eauto.
+  - etransitivity; [|symmetry; eauto];
+      etransitivity; [eauto|]; eauto.
+Qed.
+
+Lemma context_renumbered_1 f ctxt ctx ctxt' ctx' t
+      (x : interp_type t) :
+  context_renumbered f ctxt ctx ctxt' ctx' ->
+  context_renumbered (offset_renumbering 1 f)
+                     (t * ctxt) (x, ctx) (t * ctxt') (x, ctx').
+Proof.
+  cbv [context_renumbered].
+  intros ? n u.
+  destruct n; cbn [lookup offset_renumbering optsub].
+  - reflexivity.
+  - rewrite Nat.add_1_l.
+    cbn [lookup].
+    eauto.
+Qed.
+
+Lemma lookup_renumber_ref ctxt ctx ctxt' ctx' f r t :
+  context_renumbered f ctxt ctx ctxt' ctx' ->
+  lookup_ref ctxt' ctx' (renumber_ref f r) t =
+  lookup_ref ctxt ctx r t.
+Proof.
+  cbv [context_renumbered].
+  intros.
+  revert t; induction r; intros t; cbn [lookup_ref renumber_ref]; eauto.
+  destruct t; eauto.
+  rewrite IHr1, IHr2.
+  reflexivity.
+Qed.
+
+Lemma interp_op_renumber n f o ctxt ctx ctxt' ctx' tk
+      (k k' : forall ctxt, interp_type ctxt -> M tk) :
+  context_renumbered (offset_renumbering n f) ctxt ctx ctxt' ctx' ->
+  continuation_renumbered (offset_renumbering (n + 1) f) tk k k' ->
+  Mequiv
+    (Mbind (interp_op_silent ctxt ctx o)
+       (fun x : interp_type (op_type o) =>
+        k (op_type o * ctxt)%etype (x, ctx)))
+    (Mbind
+       (interp_op_silent ctxt' ctx'
+          (renumber_op (offset_renumbering n f) o))
+       (fun
+          x : interp_type
+                (op_type
+                   (renumber_op (offset_renumbering n f) o)) =>
+        k'
+          (op_type (renumber_op (offset_renumbering n f) o) *
+           ctxt')%etype (x, ctx'))).
+Proof.
+  intros Hctx Hk.
+  destruct o; cbn [renumber_op op_type];
+    (eapply Mequiv_Mbind;
+     [|intros;
+       eapply Hk;
+       rewrite plus_comm;
+       rewrite context_renumbered_ext by
+           (eauto using offset_renumbering_plus);
+       eapply context_renumbered_1; eauto]).
+  - reflexivity.
+  - cbv [interp_op_silent interp_op].
+    erewrite lookup_renumber_ref by eauto.
+    reflexivity.
+  - cbv [interp_op_silent interp_op].
+    erewrite lookup_renumber_ref by eauto.
+    reflexivity.
+Qed.
+
+Lemma interp_renumbered_bindings (f : nat -> nat)
+      (p : list operation)
+      tk (k k' : forall ctxt : type, interp_type ctxt -> M tk) :
+  continuation_renumbered (offset_renumbering (length p) f) tk k k' ->
+  continuation_renumbered
+    f tk
+    (fun ctxt ctx => interp_bindings ctxt ctx p tk k)
+    (fun ctxt ctx => interp_bindings ctxt ctx (renumber_bindings f p) tk k').
+Proof.
+  revert tk k k'.
+  pattern p; eapply rev_ind;
+    cbn [renumber_bindings interp_bindings length offset_renumbering
+                           optsub plus]; eauto.
+  clear p.
+  intros o p IHp tk k k' Hkk'.
+  rewrite app_length in Hkk'; cbn [length] in Hkk'.
+  rewrite renumber_bindings_app.
+  cbn [renumber_bindings].
+  setoid_rewrite interp_bindings_app.
+  eapply IHp.
+  cbn [interp_bindings].
+  intros ctxt ctx ctxt' ctx' Hctx'.
+  eapply interp_op_renumber; eauto.
+Qed.
